Mechanism to detect decidable atoms

src/cdcl.ml
@@ -2,9 +2,10 @@ open Names
 open Constr
 module P = ProverPatch
 
-let constr_of_ref str =
-  EConstr.of_constr (UnivGen.constr_of_monomorphic_global (Coqlib.lib_ref str))
+let constr_of_gref r =
+  EConstr.of_constr (UnivGen.constr_of_monomorphic_global r)
 
+let constr_of_ref str = constr_of_gref (Coqlib.lib_ref str)
 let coq_True = lazy (Coqlib.lib_ref "core.True.type")
 let coq_False = lazy (Coqlib.lib_ref "core.False.type")
 let coq_and = lazy (Coqlib.lib_ref "core.and.type")
@@ -27,6 +28,14 @@ let coq_false = lazy (constr_of_ref "core.bool.false")
 let coq_int = lazy (constr_of_ref "num.int63.type")
 
 (* Evaluation *)
+let coq_eval_is_dec = lazy (constr_of_ref "cdcl.eval_is_dec")
+let coq_dProp = lazy (constr_of_ref "cdcl.dProp")
+let coq_DecP1 = lazy (constr_of_ref "cdcl.DecP1")
+let coq_DecP2 = lazy (constr_of_ref "cdcl.DecP2")
+let coq_decP1 = lazy (constr_of_ref "cdcl.decP1")
+let coq_decP2 = lazy (constr_of_ref "cdcl.decP2")
+let coq_mkAtom = lazy (constr_of_ref "cdcl.mkAtom")
+let coq_mkDecAtom = lazy (constr_of_ref "cdcl.mkDecAtom")
 let coq_eval_prop = lazy (constr_of_ref "cdcl.eval_prop")
 let coq_eval_hformula = lazy (constr_of_ref "cdcl.eval_hformula")
 let coq_empty = lazy (constr_of_ref "cdcl.IntMap.empty")
@@ -36,56 +45,104 @@ let is_prop env sigma term =
   let sort = Retyping.get_sort_of env sigma term in
   Sorts.is_prop sort
 
-module Env = struct
-  type gl = {env : Environ.env; sigma : Evd.evar_map}
+module IMap = Map.Make (Int)
 
+module Env = struct
   module OMap = Map.Make (struct
     type t = P.op * Uint63.t * Uint63.t
 
     let compare : t -> t -> int = Pervasives.compare
   end)
 
+  module AMap = Map.Make (Int)
+
+  type dec = NotDec | IsDec of EConstr.t (* Proof of p \/ ~ p *)
+
+  let is_dec = function NotDec -> false | IsDec _ -> true
+
   type t =
     { fresh : int
-    ; vars : (EConstr.t * int) list (* hcons value for atoms *)
+    ; vars : (EConstr.t * (int * dec)) list (* hcons value for atoms *)
+    ; amap : (EConstr.t * dec) AMap.t (* same as vars + is_dec*)
     ; hmap : int OMap.t
-    ; gl : gl }
+    ; sigma : Evd.evar_map }
 
-  let empty gl =
+  let get_constr_of_atom ep a =
+    ProverPatch.(
+      match a.HCons.elt with
+      | AT i -> (fst (AMap.find (Uint63.hash i) ep.amap), Uint63.hash i)
+      | _ -> raise Not_found)
+
+  let empty sigma =
     { fresh = 2
     ; (* 0,1 are reserved for false and true *)
       vars = []
+    ; amap = AMap.empty
     ; hmap = OMap.empty
-    ; gl }
+    ; sigma }
 
   (** [eq_constr gl x y] returns an updated [gl] if x and y can be unified *)
-  let eq_constr gl x y =
-    let evd = gl.sigma in
-    match EConstr.eq_constr_universes_proj gl.env evd x y with
+  let eq_constr (env, sigma) x y =
+    match EConstr.eq_constr_universes_proj env sigma x y with
     | Some csts -> (
       let csts =
-        UnivProblem.to_constraints ~force_weak:false (Evd.universes evd) csts
+        UnivProblem.to_constraints ~force_weak:false (Evd.universes sigma) csts
       in
-      match Evd.add_constraints evd csts with
-      | evd -> Some {gl with sigma = evd}
+      match Evd.add_constraints sigma csts with
+      | evd -> Some sigma
       | exception Univ.UniverseInconsistency _ -> None )
     | None -> None
 
-  let hcons_atom env v =
-    let rec find gl v vars =
+  let is_dec_constr env evd t =
+    match EConstr.kind evd t with
+    | App (c, a) -> (
+      let len = Array.length a in
+      if len = 1 then
+        (* Unary predicate *)
+        let ty = Retyping.get_type_of env evd a.(0) in
+        let tc = EConstr.mkApp (Lazy.force coq_DecP1, [|ty; c|]) in
+        try
+          let _evd, dec = Typeclasses.resolve_one_typeclass env evd tc in
+          IsDec (EConstr.mkApp (Lazy.force coq_decP1, [|ty; c; dec; a.(1)|]))
+        with Not_found -> NotDec
+      else
+        let c, v1, v2 =
+          if len = 2 then (c, a.(0), a.(1))
+          else
+            ( EConstr.mkApp (c, Array.sub a 0 (Array.length a - 2))
+            , a.(len - 2)
+            , a.(len - 1) )
+        in
+        let ty1 = Retyping.get_type_of env evd v1 in
+        let ty2 = Retyping.get_type_of env evd v2 in
+        let tc = EConstr.mkApp (Lazy.force coq_DecP2, [|ty1; ty2; c|]) in
+        try
+          let _evd, dec = Typeclasses.resolve_one_typeclass env evd tc in
+          IsDec
+            (EConstr.mkApp (Lazy.force coq_decP2, [|ty1; ty2; c; dec; v1; v2|]))
+        with Not_found -> NotDec )
+    | _ -> NotDec
+
+  let hcons_atom genv env v =
+    let rec find sigma v vars =
       match vars with
       | [] -> raise Not_found
       | (e, i) :: vars -> (
-        match eq_constr gl e v with
-        | Some gl' -> (gl', i)
-        | None -> find gl v vars )
+        match eq_constr (genv, sigma) e v with
+        | Some sigma' -> (sigma', i)
+        | None -> find sigma v vars )
     in
     try
-      let gl', i = find env.gl v env.vars in
-      ({env with gl = gl'}, i)
+      let sigma', i = find env.sigma v env.vars in
+      ({env with sigma = sigma'}, i)
     with Not_found ->
+      let dec = is_dec_constr genv env.sigma v in
       let f = env.fresh in
-      ({env with vars = (v, f) :: env.vars; fresh = f + 1}, f)
+      ( { env with
+          vars = (v, (f, dec)) :: env.vars
+        ; amap = AMap.add f (v, dec) env.amap
+        ; fresh = f + 1 }
+      , (f, dec) )
 
   let hcons_op env op f1 f2 =
     try (env, OMap.find (op, f1, f2) env.hmap)
@@ -96,23 +153,30 @@ module Env = struct
       , env.fresh )
 
   let map_of_env env =
+    let add = Lazy.force coq_add in
+    let ty = Lazy.force coq_dProp in
+    let mk_atom = Lazy.force coq_mkAtom in
+    let mk_dec_atom = Lazy.force coq_mkDecAtom in
+    let mk_atom (p, d) =
+      match d with
+      | NotDec -> EConstr.mkApp (mk_atom, [|p|])
+      | IsDec prf -> EConstr.mkApp (mk_dec_atom, [|p; prf|])
+    in
     let add i e m =
-      EConstr.mkApp
-        ( Lazy.force coq_add
-        , [|EConstr.mkProp; EConstr.mkInt (Uint63.of_int i); e; m|] )
+      EConstr.mkApp (add, [|ty; EConstr.mkInt (Uint63.of_int i); mk_atom e; m|])
     in
     let rec map_of_list l =
       match l with
-      | [] -> EConstr.mkApp (Lazy.force coq_empty, [|EConstr.mkProp|])
-      | (e, i) :: l -> add i e (map_of_list l)
+      | [] -> EConstr.mkApp (Lazy.force coq_empty, [|ty|])
+      | (e, (i, d)) :: l -> add i (e, d) (map_of_list l)
     in
     map_of_list env.vars
 end
 
 let hcons i b f = P.HCons.{id = Uint63.of_int i; is_dec = b; elt = f}
 
-let reify_formula env (f : EConstr.t) =
-  let evd = env.Env.gl.Env.sigma in
+let reify_formula genv env (f : EConstr.t) =
+  let evd = env.Env.sigma in
   let tt = hcons 1 true P.TT in
   let ff = hcons 0 true P.FF in
   let mkop o f1 f2 = P.OP (o, f1, f2) in
@@ -122,8 +186,8 @@ let reify_formula env (f : EConstr.t) =
   let is_and = eq_ind (Lazy.force coq_and) in
   let is_or = eq_ind (Lazy.force coq_or) in
   let var env f =
-    let env', i = Env.hcons_atom env f in
-    (hcons i false (P.AT (Uint63.of_int i)), env')
+    let env', (i, dec) = Env.hcons_atom genv env f in
+    (hcons i (Env.is_dec dec) (P.AT (Uint63.of_int i)), env')
   in
   let get_binop t =
     match EConstr.kind evd t with
@@ -155,19 +219,19 @@ let reify_formula env (f : EConstr.t) =
   in
   reify_formula env f
 
-let rec reify_hyps env (hyps : (Names.Id.t * EConstr.types) list) =
+let rec reify_hyps genv env (hyps : (Names.Id.t * EConstr.types) list) =
   match hyps with
   | [] -> ([], env)
   | (id, t) :: l ->
-    let lhyps, env = reify_hyps env l in
-    if is_prop env.Env.gl.Env.env env.Env.gl.Env.sigma t then
-      let hf, env = reify_formula env t in
+    let lhyps, env = reify_hyps genv env l in
+    if is_prop genv env.Env.sigma t then
+      let hf, env = reify_formula genv env t in
       ((id, hf) :: lhyps, env)
     else (lhyps, env)
 
-let reify_goal env hyps concl =
-  let hyps, env = reify_hyps env hyps in
-  let hf, env = reify_formula env concl in
+let reify_goal genv env hyps concl =
+  let hyps, env = reify_hyps genv env hyps in
+  let hf, env = reify_formula genv env concl in
   (hyps, hf, env)
 
 let make_formula env hyps hconcl =
@@ -232,26 +296,153 @@ let nat_of_int i =
     let rec nat_of_int i = if i = 0 then P.O else P.S (nat_of_int (i - 1)) in
     nat_of_int i
 
-(*let lia_prover env clause =*)
+module Theory = struct
+  open ProverPatch
+  open Micromega_plugin
+  module Mc = Micromega
 
-let run_prover f = ()
+  let rec parse_clause (genv, sigma) ep env l =
+    match l with
+    | [] -> (Mc.FF Mc.IsProp, env)
+    | a :: l -> (
+      let f, env = parse_clause (genv, sigma) ep env l in
+      try
+        let form = form_of_literal a in
+        let eform, i = Env.get_constr_of_atom ep form in
+        let at, env =
+          Coq_micromega.parse_zarith Mc.IsProp env eform (genv, sigma)
+        in
+        let at = Mc.A (Mc.IsProp, at, i) in
+        match a with
+        | POS _ -> (Mc.OR (Mc.IsProp, at, f), env)
+        | NEG _ -> (Mc.IMPL (Mc.IsProp, at, None, f), env)
+      with Not_found | Coq_micromega.ParseError | Failure _ -> (f, env) )
 
-(*  let m = P.hcons_form f in
-  ignore (P.prover_formula Uint63.equal (fun _ -> false) m (nat_of_int 200) f);
-  Printf.printf "\nrun prover done\n";
-  flush stdout
- *)
+  open Coq_micromega
+  open Certificate
+
+  let iset_of_list l =
+    List.fold_left (fun acc i -> Mutils.ISet.add i acc) Mutils.ISet.empty l
+
+  let map_of_list l =
+    let rec map_of_list m i l =
+      match l with
+      | [] -> m
+      | (_, id) :: l -> map_of_list (IMap.add i id m) (i + 1) l
+    in
+    map_of_list IMap.empty 0 l
+
+  let find_deps_of_prf p prf l =
+    let m = map_of_list l in
+    let hyps = p.hyps prf in
+    Mutils.ISet.fold
+      (fun i acc -> Mutils.ISet.add (IMap.find i m) acc)
+      hyps Mutils.ISet.empty
+
+  let find_unsat_clause p clid =
+    let cl = List.map fst clid in
+    match p.prover (p.get_option (), cl) with
+    | Model _ -> None
+    | Unknown -> None
+    | Prf prf -> Some (find_deps_of_prf p prf clid)
+
+  let rec find_unsat_core p s l =
+    match l with
+    | [] -> Some s
+    | cl :: l -> (
+      match find_unsat_clause p cl with
+      | None -> None
+      | Some s' -> find_unsat_core p (Mutils.ISet.union s s') l )
+
+  let select_atom is lit =
+    let id = Uint63.hash (form_of_literal lit).HCons.id in
+    Mutils.ISet.mem id is
+
+  let thy_prover cc p (genv, sigma) ep hm l =
+    let env = Coq_micromega.Env.empty (genv, sigma) in
+    let cl, _ = parse_clause (genv, sigma) ep env l in
+    let cnf_ff, cnf_ff_tags = Mc.cnfZ Mc.IsProp cl in
+    match find_unsat_core p (iset_of_list cnf_ff_tags) cnf_ff with
+    | None ->
+      Printf.fprintf stdout "Thy ⊬ %a\n" P.output_literal_list l;
+      None
+    | Some is ->
+      let c = List.filter (select_atom is) l in
+      Printf.fprintf stdout "Thy ⊢ %a\n" P.output_literal_list c;
+      cc := c :: !cc;
+      Some (hm, c)
+end
+
+let run_prover cc (genv, sigma) ep f =
+  let is_dec i =
+    try
+      let c, d = Env.AMap.find (Uint63.hash i) ep.Env.amap in
+      Env.is_dec d
+    with Not_found -> false
+  in
+  let m = P.hcons_form f in
+  P.prover_formula Uint63.equal is_dec
+    (Theory.thy_prover cc Micromega_plugin.Coq_micromega.linear_Z (genv, sigma)
+       ep)
+    true m (nat_of_int 200) f
+
+let constr_of_literal_list ep mkFF mkOr mkImpl l =
+  P.(
+    let rec constr_of_literal_list l =
+      match l with
+      | [] -> mkFF
+      | x :: l ->
+        (match x with POS a -> mkOr | NEG a -> mkImpl)
+          (fst (Env.get_constr_of_atom ep (P.form_of_literal x)))
+          (constr_of_literal_list l)
+    in
+    constr_of_literal_list l)
+
+let fresh_id id gl =
+  Tactics.fresh_id_in_env Id.Set.empty id (Proofview.Goal.env gl)
+
+let assert_conflicts ep l tac gl =
+  let mkFF = constr_of_gref (Lazy.force coq_False) in
+  let mkOr x y = EConstr.mkApp (constr_of_gref (Lazy.force coq_or), [|x; y|]) in
+  let mkImpl x y = EConstr.mkArrow x Sorts.Irrelevant y in
+  let mk_goal c = constr_of_literal_list ep mkFF mkOr mkImpl c in
+  let rec assert_conflicts n l =
+    match l with
+    | [] -> Tacticals.New.tclIDTAC
+    | c :: l ->
+      let id = fresh_id (Names.Id.of_string ("__arith" ^ string_of_int n)) gl in
+      Tacticals.New.tclTHEN
+        (Tactics.assert_by (Names.Name id) (mk_goal c) tac)
+        (assert_conflicts (n + 1) l)
+  in
+  assert_conflicts 0 l
+
+(** [assert_conflicts_clauses tac] runs the sat prover in ml 
+    and asserts conflict_clauses *)
+let assert_conflicts_clauses tac =
+  Proofview.Goal.enter (fun gl ->
+      Coqlib.check_required_library ["Cdcl"; "Formula"];
+      let sigma = Tacmach.New.project gl in
+      let genv = Tacmach.New.pf_env gl in
+      let concl = Tacmach.New.pf_concl gl in
+      let hyps = Tacmach.New.pf_hyps_types gl in
+      let hyps, concl, env = reify_goal genv (Env.empty sigma) hyps concl in
+      let form, env = make_formula env (List.rev hyps) concl in
+      let cc = ref [] in
+      match run_prover cc (genv, sigma) env form with
+      | P.HasProof _ -> assert_conflicts env !cc tac gl
+      | _ -> Tacticals.New.tclFAIL 0 (Pp.str "Not a tautology"))
+
 let change_goal =
   Proofview.Goal.enter (fun gl ->
       Coqlib.check_required_library ["Cdcl"; "Formula"];
       let sigma = Tacmach.New.project gl in
+      let genv = Tacmach.New.pf_env gl in
       let concl = Tacmach.New.pf_concl gl in
       let hyps = Tacmach.New.pf_hyps_types gl in
-      let gl0 = {Env.env = Tacmach.New.pf_env gl; sigma} in
       let typ = Lazy.force coq_int in
-      let hyps, concl, env = reify_goal (Env.empty gl0) hyps concl in
+      let hyps, concl, env = reify_goal genv (Env.empty sigma) hyps concl in
       let form, env = make_formula env (List.rev hyps) concl in
-      ignore (run_prover form);
       let cform = constr_of_formula typ form in
       let m = Env.map_of_env env in
       Tacticals.New.tclTHEN
@@ -262,3 +453,5 @@ let change_goal =
               ( Lazy.force coq_eval_hformula
               , [|typ; EConstr.mkApp (Lazy.force coq_eval_prop, [|m|]); cform|]
               ))))
+
+let cdcl tac = Tacticals.New.tclTHEN (assert_conflicts_clauses tac) change_goal
